WIP

security/Backtranslation.v
@@ -1310,13 +1310,18 @@ Section Backtranslation.
     Definition match_params pars (ge_c: genv) (ge_i: Asm.genv) :=
       (wf_params_of pars) /\ (wf_params_of_sig pars ge_i) /\ (wf_params_of_symb pars ge_c).
 
+    Definition match_cnts cnts (ge_c: genv) (k: meminj) :=
+      forall id cnt cnt_b, (cnts ! id = Some cnt) -> (Genv.find_symbol ge_c cnt = Some cnt_b) ->
+                      (forall b ofs, k b <> Some (cnt_b, ofs)).
+
     Definition match_state (ge_i: Asm.genv) (ge_c: Clight.genv) (k: meminj) tr cnts pars id (ist: ir_state) (cst: Clight.state) :=
       match ist, cst with
       | Some (cur, m_i, k_i), State f _ k_c e le m_c =>
           (match_genv ge_i ge_c) /\ (match_mem ge_i k m_i m_c) /\
             (match_cur_fun ge_i ge_c cur f id) /\ (match_find_def ge_i ge_c cnts pars tr) /\
             (match_cont ge_c tr cnts k_c k_i) /\
-            (match_params pars ge_c ge_i)
+            (match_params pars ge_c ge_i) /\
+            (match_cnts cnts ge_c k)
       | _, _ => False
       end.
 
@@ -2382,7 +2387,36 @@ Section Backtranslation.
       ss. eapply Mem.free_unchanged_on. eapply Heq. ii. apply H0; clear H0. left; auto.
     Qed.
 
+    Lemma mem_inject_incr_match_cnts_rev
+          k1 k2
+          (INCR: inject_incr k1 k2)
+          cnts ge
+          (MC: match_cnts cnts ge k2)
+      :
+      match_cnts cnts ge k1.
+    Proof.
+      unfold match_cnts in *. i. specialize (MC _ _ _ H H0 b ofs). ii. apply MC; clear MC. apply INCR. auto.
+    Qed.
 
+    Lemma star_cut_middle
+          stepk ge_c cst1 ev pretr ttr cnts ge_i pars ist2
+          (CUT: exists tr1 cst',
+              (star stepk ge_c cst1 tr1 cst') /\
+                exists tr2 cst2,
+                  (star stepk ge_c cst' tr2 cst2) /\
+                    ((exists id', (wf_c_state ge_c (pretr ++ [ev]) ttr cnts id' cst2) /\
+                               exists k, (match_state ge_i ge_c k ttr cnts pars id' ist2 cst2))
+                     \/ (ist2 = None)) /\
+                    (unbundle ev = tr1 ++ tr2))
+      :
+      exists cst2, (star stepk ge_c cst1 (unbundle ev) cst2) /\
+                ((exists id', (wf_c_state ge_c (pretr ++ [ev]) ttr cnts id' cst2) /\
+                           exists k, (match_state ge_i ge_c k ttr cnts pars id' ist2 cst2))
+                 \/ (ist2 = None)).
+    Proof.
+      destruct CUT as (tr1 & cts' & STAR1 & tr2 & cst2 & STAR2 & PROP & TR).
+      exists cst2. split; auto. eapply star_trans. eapply STAR1. eapply STAR2. auto.
+    Qed.
 
 
 
@@ -2409,7 +2443,7 @@ Section Backtranslation.
       unfold wf_c_state in WFC. des_ifs. rename s into stmt, k into k_c, m into m_c.
       destruct WFC as ((CNT_INJ & WFC0) & (m_freeenv & FREEENV & WFC1) & WFC2 & WFC3 & WFC4 & WFNB).
       unfold match_state in MS. des_ifs. rename i into k_i, b into cur, m into m_i.
-      destruct MS as (MS0 & MS1 & MS2 & MS3 & MS4 & MS5).
+      destruct MS as (MS0 & MS1 & MS2 & MS3 & MS4 & MS5 & MCNTS).
       move STEP after WFC4. inv STEP.
 
       - assert (id = id_cur).
@@ -2618,14 +2652,14 @@ Section Backtranslation.
               eapply alloc_variables_mem_inject. eapply ENV_ALLOC. auto.
             + move MS1 after ENV_NINJ. destruct MS1 as (MM1 & MM2 & MM3).
               move DELTA after ENV_NINJ. eapply meminj_not_alloc_delta. eapply MM3. eapply DELTA.
-
           - unfold match_cur_fun. splits; auto.
             + rewrite Genv.find_funct_ptr_iff. eapply FINDF_C.
             + eexists. eapply FINDF.
             + apply Genv.find_invert_symbol. apply FINDB.
-
           - move MS4 after ENV_NINJ. econs 2. 4,5,6: eauto. all: auto.
             apply Genv.find_invert_symbol. apply FIND_CUR_C.
+          - move MS1 after ENV_NINJ. move MCNTS after MS1. destruct MS1 as (MM1 & MM2 & MM3).
+            eapply mem_inject_incr_match_cnts_rev. eapply MM2. auto.
         }
         exists cst2. split.
         2:{ left. exists id_next. split. apply WFC_NEXT. eexists. eapply MS_NEXT. }
@@ -2841,17 +2875,27 @@ Section Backtranslation.
             eapply wunchanged_on_nextblock in CNT_CUR_STORE, DELTA_C.
             clear - WFNB CNT_CUR_STORE DELTA_C.
             do 5 (etransitivity; eauto).
+            Unshelve. all: try (exact 0%nat). all: try (exact (fun _ _ => True)).
         }
 
         assert (MS_NEXT: match_state ge_i ge_c (meminj_public ge_i) ttr cnts pars id_next (Some (b, m2, ik')) cst2).
-        {
-
-
-
-          TODO
-
-          admit. }
-
+        { clear CUR_SWITCH_STAR WFC_NEXT. ss. splits; auto.
+          - unfold match_mem. splits; auto.
+            + eapply SimplLocalsproof.free_list_right_inject. eapply MEMINJ_CNT. eapply FREENEXT.
+              i. move WFC4 after cst2. apply not_global_is_not_inj_bloks in WFC4. setoid_rewrite Forall_forall in WFC4.
+              assert (b2 = b1).
+              { clear - H. unfold meminj_public in H. des_ifs. }
+              subst b2. hexploit (WFC4 b1).
+              { unfold blocks_of_env2, blocks_of_env in *. rewrite map_map.
+                eapply (in_map (fun x => fst (fst x))) in H0. ss. rewrite map_map in H0. ss.
+              }
+              intros. erewrite <- match_symbs_meminj_public in H3. rewrite H in H3. clarify.
+              destruct MS0 as (MS & _). apply MS.
+            + move MS1 after cst2. destruct MS1 as (MM1 & MM2 & MM3).
+              move DELTA after cst2. eapply meminj_not_alloc_delta. eapply MM3. eapply DELTA.
+          - unfold match_cur_fun. splits; auto. eauto.
+          - destruct MS1 as (MM1 & MM2 & MM3). eapply mem_inject_incr_match_cnts_rev; eauto.
+        }
         exists cst2. split.
         2:{ left. exists id_next. split. apply WFC_NEXT. eexists. eapply MS_NEXT. }
 
@@ -2906,7 +2950,579 @@ Section Backtranslation.
         }
         all: traceEq. traceEq.
 
-      -
+      - assert (id = id_cur).
+        { unfold match_cur_fun in MS2. desH MS2. rewrite MS7 in IDCUR. clarify. }
+        subst id. rename id0 into id_next. 
+
+        set (pretr ++ (id_cur, Bundle_call tr id_next (vals_to_eventvals ge_i vargs) (ef_sig ef) d) :: btr) as ttr in *.
+        assert (FIND_CUR_C: Genv.find_symbol ge_c id_cur = Some cur).
+        { destruct MS0 as ((MSENV0 & MSENV1 & MSENV2) & MGENV). apply Genv.invert_find_symbol in IDCUR. apply MSENV1 in IDCUR. auto. }
+        assert (FIND_FUN_C: Genv.find_funct_ptr ge_c cur = Some (Internal f)).
+        { destruct MS2 as (MFUN0 & MFUN1). auto. }
+
+        exploit WFC0. eapply FIND_CUR_C. eapply FIND_FUN_C. intros (cnt_cur & CNTS_CUR & WF_CNT_CUR).
+        assert (CUR_TR: get_id_tr ttr id_cur = (get_id_tr pretr id_cur) ++ (id_cur, Bundle_call tr id_next (vals_to_eventvals ge_i vargs) (ef_sig ef) d) :: (get_id_tr btr id_cur)).
+        { subst ttr. clear. rewrite get_id_tr_app. rewrite get_id_tr_cons. ss. rewrite Pos.eqb_refl. auto. }
+        assert (BOUND2: Z.of_nat (Datatypes.length (map (fun ib : ident * bundle_event => code_bundle_event ge_i (comp_of f) (snd ib)) (get_id_tr ttr id_cur))) < Int64.modulus).
+        { rewrite map_length. etransitivity. 2: eauto. unfold get_id_tr. admit. (* ez *) }
+        destruct WF_CNT_CUR as (CNT_CUR_NPUB & cnt_cur_b & FIND_CNT_CUR & CNT_CUR_MEM_VA & CNT_CUR_MEM_LOAD).
+
+        destruct MS2 as (FINDF_C_CUR & (f_i_cur & FINDF_I_CUR) & INV_CUR).
+        hexploit cur_fun_def. eapply FINDF_C_CUR. eapply FINDF_I_CUR. eapply INV_CUR. eauto.
+        intros (cnt_cur0 & params_cur & CNT_CUR0 & PARAMS_CUR & CUR_F).
+        rewrite CNTS_CUR in CNT_CUR0. inversion CNT_CUR0. subst cnt_cur0. clear CNT_CUR0.
+        assert (CP_CUR: (comp_of f) = (Genv.find_comp ge_i (Vptr cur Ptrofs.zero))).
+        { unfold Genv.find_comp. setoid_rewrite FINDF_I_CUR. subst f. ss. }
+
+        hexploit switch_spec.
+        { subst ttr. rewrite CUR_TR in BOUND2. rewrite map_app in BOUND2. ss. eapply BOUND2. }
+        { unfold wf_env in WFC3. specialize (WFC3 cnt_cur). des_ifs. eapply WFC3. }
+        eapply FIND_CNT_CUR. eapply CNT_CUR_MEM_VA.
+        { rewrite CNT_CUR_MEM_LOAD. rewrite map_length. auto. }
+        instantiate (1:=le).
+        instantiate (1:= (Kloop1 (Ssequence (Sifthenelse one_expr Sskip Sbreak) (switch_bundle_events ge_c cnt_cur (comp_of f) (get_id_tr ttr id_cur))) Sskip k0)).
+        instantiate (1:=Sreturn None).
+        intros (m_cu & CNT_CUR_STORE & CUR_SWITCH_STAR).
+        rename MEM into DELTA. move ECCASES after CUR_SWITCH_STAR.
+        desH ECCASES; cycle 1.
+
+        { subst d. unfold mem_delta_apply_wf in DELTA. simpl in DELTA. inversion DELTA; clear DELTA. subst m1'.
+
+          Lemma exists_vargs_vres
+                (ge1: Senv.t) (ge2: genv)
+                (MS: match_symbs ge1 ge2)
+                ef m1 vargs tr vretv m2
+                (EK: external_call_known_observables ef ge1 m1 vargs tr vretv m2)
+                e cp le m_c
+                (WFE: wf_env ge2 e)
+            :
+            exists vargs2 vretv2,
+              (eval_exprlist ge2 e cp le m_c (list_eventval_to_list_expr (vals_to_eventvals ge1 vargs))
+                             (list_typ_to_typelist (sig_args (ef_sig ef))) vargs2) /\
+                (external_call ef ge2 vargs2 m_c tr vretv2 m_c).
+          Proof.
+            pose proof MS as MS0. destruct MS as (MS1 & MS2 & MS3). move MS0 after MS1.
+            unfold external_call_known_observables in *. des_ifs; ss; des. all: try (inv EK; clarify; ss).
+            - inv H; clarify. unfold senv_invert_symbol_total. hexploit Senv.find_invert_symbol; eauto. intros INV. rewrite INV.
+              esplits.
+              + econs. 3: econs. eapply ptr_of_id_ofs_eval; eauto. rewrite ptr_of_id_ofs_typeof. apply sem_cast_ptr.
+              + econs. econs; auto. rewrite MS3; auto. eapply match_symbs_eventval_match; eauto.
+            - inv H; clarify. unfold senv_invert_symbol_total. hexploit Senv.find_invert_symbol; eauto. intros INV. rewrite INV.
+              esplits.
+              + econs. eapply ptr_of_id_ofs_eval; eauto. rewrite ptr_of_id_ofs_typeof. apply sem_cast_ptr.
+                econs. 3: econs.
+                { instantiate (1:=v). destruct v; ss; try (econs; fail).
+                  - destruct chunk; ss; inv H2; ss.
+                  - destruct Archi.ptr64 eqn:ARCH.
+                    + destruct chunk; ss; inv H2; ss; des_ifs.
+                      * unfold senv_invert_symbol_total. hexploit Senv.find_invert_symbol. eapply H6. intros INV2. rewrite INV2.
+                        eapply ptr_of_id_ofs_eval; eauto.
+                      * unfold senv_invert_symbol_total. hexploit Senv.find_invert_symbol. eapply H7. intros INV2. rewrite INV2.
+                        eapply ptr_of_id_ofs_eval; eauto.
+                    + destruct chunk; ss; inv H2; ss; des_ifs.
+                      * unfold senv_invert_symbol_total. hexploit Senv.find_invert_symbol. eapply H6. intros INV2. rewrite INV2.
+                        eapply ptr_of_id_ofs_eval; eauto.
+                      * unfold senv_invert_symbol_total. hexploit Senv.find_invert_symbol. eapply H6. intros INV2. rewrite INV2.
+                        eapply ptr_of_id_ofs_eval; eauto.
+                      * unfold senv_invert_symbol_total. hexploit Senv.find_invert_symbol. eapply H7. intros INV2. rewrite INV2.
+                        eapply ptr_of_id_ofs_eval; eauto.
+                }
+                { instantiate (1:=Val.load_result chunk v).
+
+                  TODO
+
+                  
+                  destruct v; ss.
+                  - destruct chunk; ss; inv H2; ss.
+                  - destruct chunk; ss. all: simpl_expr.
+                    + inv H2.
+            - esplits.
+              + erewrite eventval_list_match_vals_to_eventvals. 2: eapply H.
+                eapply list_eventval_to_expr_val_eval; auto. eapply eventval_list_match_transl.
+                eapply match_senv_eventval_list_match; eauto.
+              + econs. eapply eventval_list_match_transl_val. eapply match_senv_eventval_list_match; eauto.
+            - esplits.
+              + econs. 3: econs.
+                * erewrite eventval_match_val_to_eventval. 2: eapply H. eapply eventval_to_expr_val_eval; auto.
+                  eapply match_senv_eventval_match; eauto.
+                * erewrite eventval_match_val_to_eventval. 2: eapply H. eapply eventval_match_sem_cast.
+                  erewrite eventval_match_eventval_to_val.
+                  eapply match_senv_eventval_match. eauto. eapply H. eapply match_senv_eventval_match. eauto. eapply H.
+              + econs. erewrite eventval_match_eventval_to_val.
+                eapply match_senv_eventval_match. eauto. eapply H. eapply match_senv_eventval_match. eauto. eapply H.
+          Qed.
+
+          eapply star_cut_middle. exists E0.
+          eexists. split.
+          { unfold wf_c_stmt in WFC2. specialize (WFC2 _ CNTS_CUR). subst stmt.
+            eapply star_trans. eapply code_bundle_trace_spec. 2: ss.
+            unfold switch_bundle_events at 1. rewrite CUR_TR at 1. rewrite map_app. simpl.
+            rewrite ! (match_symbs_code_bundle_call ge_i ge_c) in CUR_SWITCH_STAR.
+            rewrite ! (match_symbs_code_bundle_events ge_i ge_c) in CUR_SWITCH_STAR.
+            eapply star_trans. eapply CUR_SWITCH_STAR. 2: ss. 2,3: destruct MS0 as (MS & _); auto.
+            clear BOUND2 CUR_SWITCH_STAR.
+            unfold code_bundle_call. eapply star_trans. eapply code_mem_delta_correct. auto.
+            { unfold mem_delta_apply_wf. simpl. reflexivity. }
+            2: ss. econs 2. 2: econs 1. 2: traceEq.
+            eapply step_call. ss.
+            { econs. assert (FSN_C: Senv.find_symbol ge_c id_next = Some b_ext).
+              { destruct MS0 as ((MSENV0 & MSENV1 & MSENV2) & MGENV). apply MSENV1. auto. }
+              eapply eval_Evar_global.
+              - unfold wf_env in WFC3. specialize (WFC3 id_next). rewrite FSN_C in WFC3. apply WFC3.
+              - eapply FSN_C.
+              - econs 2. ss.
+            }
+            { TODO
+
+              Lemma match_symbs_extcall_known_obs
+                    ge1 ge2
+                    (MS: match_symbs ge1 ge2)
+                    ef m1 vargs tr vretv m2
+                    (EK: external_call_known_observables ef ge1 m1 vargs tr vretv m2)
+                :
+                external_call_known_observables ef ge2 m1 vargs tr vretv m2.
+              Proof.
+                pose proof MS as MS0. destruct MS as (MS1 & MS2 & MS3).
+                unfold external_call_known_observables in *. des_ifs; ss; des. all: splits; [inv EK; clarify | auto].
+                - inv H; clarify. econs. econs; auto. rewrite MS3; auto. eapply match_symbs_eventval_match; eauto.
+                - inv H; clarify. econs. econs; auto. rewrite MS3; auto. eapply match_symbs_eventval_match; eauto.
+                - econs; eauto. eapply match_symbs_eventval_list_match; eauto.
+                - econs; eauto. eapply match_symbs_eventval_match; eauto.
+              Qed.
+                             external_call ef ge vargs m t vres m' ->
+
+              (* Lemma match_symbs_vals_to_eventvals *)
+              (*       ge1 ge2 *)
+              (*       (MS: match_symbs ge1 ge2) *)
+              (*       varg *)
+              (*   : *)
+              (*   val_to_eventval ge1 varg = val_to_eventval ge2 varg. *)
+              (* Proof. *)
+              (*   destruct varg; ss. destruct MS as (MS1 & MS2 & MS3). unfold senv_invert_symbol_total. des_ifs. *)
+              (*   - apply Senv.invert_find_symbol in Heq, Heq0. apply MS2 in Heq. apply Senv.find_invert_symbol in Heq, Heq0. *)
+              (*     rewrite Heq in Heq0; clarify. *)
+              (*   - apply Senv.invert_find_symbol in Heq. apply MS2 in Heq. apply Senv.find_invert_symbol in Heq. clarify. *)
+              (*   -  *)
+              (*   -  *)
+
+              (* Lemma match_symbs_vals_to_eventvals *)
+              (*       ge1 ge2 *)
+              (*       (MS: match_symbs ge1 ge2) *)
+              (*       vargs *)
+              (*   : *)
+              (*   vals_to_eventvals ge1 vargs = vals_to_eventvals ge2 vargs. *)
+
+              Lemma extcall_known_observables_eval_args
+                    (ge0: Senv.t) (ge: genv)
+                    (MS: match_symbs ge0 ge)
+                    ef m1 vargs tr vretv m2
+                    (EK: external_call_known_observables ef ge0 m1 vargs tr vretv m2)
+                    e cp le m'
+                    (WFE : wf_env ge e)
+                :
+                eval_exprlist ge e cp le m' (list_eventval_to_list_expr (vals_to_eventvals ge0 vargs)) (list_typ_to_typelist (sig_args (ef_sig ef))) vargs.
+              Proof.
+                pose proof MS as MS0. destruct MS as (MS1 & MS2 & MS3).
+                unfold external_call_known_observables in *. des_ifs; ss; des. all: try (inv EK; clarify; ss).
+                - inv H; clarify. unfold senv_invert_symbol_total. hexploit Senv.find_invert_symbol; eauto. intros INV. rewrite INV.
+                  econs. 3: econs. eapply ptr_of_id_ofs_eval; eauto. rewrite ptr_of_id_ofs_typeof. apply sem_cast_ptr.
+                - inv H; clarify. unfold senv_invert_symbol_total. hexploit Senv.find_invert_symbol; eauto. intros INV. rewrite INV.
+                  econs.
+                  { eapply ptr_of_id_ofs_eval; eauto. }
+                  { rewrite ptr_of_id_ofs_typeof. apply sem_cast_ptr. }
+                  econs. 3: econs.
+                  { eapply val_load_result_aux in H2.  eapply eventval_to_expr_val_eval; auto. 
+                -
+
+      - inv ENV; inv EV. pose proof SEM as SEM0. inv SEM. inv H5. econstructor 2.
+        { apply val_load_result_aux in H10.
+          eapply step_builtin.
+          - econstructor; eauto. eapply ptr_of_id_ofs_eval; eauto. rewrite ptr_of_id_ofs_typeof. eapply sem_cast_ptr.
+          econstructor; eauto. 3: econstructor. eapply eventval_to_expr_val_eval; auto. eapply eventval_match_wf_eventval_ge; eauto.
+          eapply eventval_match_sem_cast. erewrite eventval_match_eventval_to_val; eauto.
+          - simpl. econstructor. econstructor 1; eauto.
+        }
+        simpl. econstructor 1. all: eauto.
+
+
+              
+            }
+            
+
+
+              eapply list_eventval_to_expr_val_eval. auto. inv TR. eapply eventval_list_match_transl. eapply match_senv_eventval_list_match; eauto. destruct MS0 as (MSENV & _); auto. }
+            { unfold match_find_def in MS3. hexploit MS3.
+              unfold Genv.find_funct in FINDF. rewrite pred_dec_true in FINDF; auto. unfold Genv.find_funct_ptr in FINDF. des_ifs. eapply Heq.
+              eapply Senv.find_invert_symbol; eapply FINDB.
+              rewrite CNTS_NEXT, PARS_NEXT. intros. unfold Genv.find_funct. rewrite pred_dec_true. unfold Genv.find_funct_ptr. rewrite H. ss. ss.
+            }
+            { ss. unfold type_of_function, gen_function. ss. f_equal. apply type_of_params_eq. apply PARSIGS. }
+            { destruct MS0 as ((MSENV0 & MSENV1 & MSENV2) & MGENV).
+              subst f. setoid_rewrite CP_CUR.
+              eapply allowed_call_gen_function; eauto.
+              { setoid_rewrite Genv.find_funct_ptr_iff. rewrite FINDF_C. subst f_next. eauto. }
+            }
+            { move NPTR after MS_NEXT. move TR after NPTR. i.
+              rewrite EVARGS. apply NPTR. unfold crossing_comp. rewrite <- H.
+              setoid_rewrite CP_CUR. rewrite CP_NEXT. auto.
+            }
+            { move TR after MS_NEXT. instantiate (1:=tr). inv TR.
+              setoid_rewrite CP_CUR. rewrite CP_NEXT.
+              econs 2.
+              { rewrite <- H. ss. }
+              eauto.
+              { destruct MS0 as ((MSENV0 & MSENV1 & MSENV2) & MGENV). apply Genv.find_invert_symbol. apply MSENV1. auto. }
+              { eapply eventval_list_match_transl. eapply match_senv_eventval_list_match; eauto. destruct MS0 as (MSENV & _); auto. }
+            }
+          }
+
+
+
+
+            eapply step_call; simpl.
+            - ss.
+            - ec
+
+
+            
+
+
+
+
+
+          
+        }
+        clear BOUND2 CUR_SWITCH_STAR.
+
+
+        assert (f1 = f_next).
+        { rewrite <- Genv.find_funct_ptr_iff in FINDF_C. rewrite FINDF_C in FUN. clarify. }
+        subst f1. clear INV_CUR.
+        assert (id = id_next).
+        { apply Genv.invert_find_symbol in INV_ID_NEXT. destruct MS0 as ((_ & MS & _) & _). apply MS in INV_ID_NEXT.
+          apply Senv.find_invert_symbol in INV_ID_NEXT. setoid_rewrite INV_ID_NEXT in ID. clarify.
+        }
+        subst id.
+        assert (cnt = cnt_next).
+        { rewrite CNTS_NEXT in CNT. clarify. }
+        subst cnt. clear ID CNT.
+
+        assert (WCHG1: wunchanged_on (fun b _ => Mem.valid_block m_c b) m_c m_c').
+        { eapply wunchanged_on_trans. eapply store_wunchanged_on. eapply CNT_CUR_STORE.
+          eapply wunchanged_on_implies. eapply mem_delta_apply_wf_wunchanged_on. eapply DELTA_C. ss.
+        }
+        assert (FREENEXT: exists m_c_next, Mem.free_list m_c' (blocks_of_env ge_c e) (comp_of f) = Some m_c_next).
+        { eapply wunchanged_on_exists_mem_free_list. eapply WCHG1. eapply FREEENV. }
+        des.
+
+        set (State f_next (fn_body f_next) ck_next e_next le_next m_c_next) as cst2.
+
+        assert (WFC_NEXT: wf_c_state ge_c (pretr ++ [(id_cur, Bundle_return tr evretv d)]) ttr cnts id_next cst2).
+        { clear CUR_SWITCH_STAR. ss. splits; auto.
+          - unfold wf_counters. split. auto.
+            move WFC0 after cst2.
+            ii. specialize (WFC0 _ _ _ H H0). des. exists cnt. splits; auto.
+            unfold wf_counter in WFC1. des. unfold wf_counter. splits; auto.
+            exists b1. splits; auto.
+            + eapply mem_valid_access_wunchanged_on. eapply WFC6.
+              eapply wunchanged_on_trans; cycle 1. eapply mem_free_list_wunchanged_on_2. eapply FREENEXT.
+              eapply wunchanged_on_trans; cycle 1. eapply mem_delta_apply_wf_wunchanged_on. eapply DELTA_C.
+              eapply store_wunchanged_on. eapply CNT_CUR_STORE. ss. i.
+              move MS5 after H0. destruct MS5 as (MP0 & MP1 & MP). specialize (MP _ _ WFC5). move WFC4 after MP.
+              eapply not_global_blks_global_not_in; eauto.
+            + move WFNB after CP_CUR. move WFC4 after WFNB.
+              eapply Mem.load_unchanged_on. eapply mem_free_list_unchanged_on. eapply FREENEXT.
+              { ss. i. eapply not_global_blks_global_not_in; eauto. }
+              erewrite mem_delta_apply_wf_mem_load; cycle 1.
+              { erewrite match_symbs_mem_delta_apply_wf in DELTA_C. apply DELTA_C. destruct MS0 as (MS & _). eauto. }
+              { eapply Genv.find_invert_symbol. apply WFC5. }
+              { auto. }
+              destruct (Pos.eq_dec id id_cur).
+              * subst id. assert (cnt_cur = cnt).
+                { rewrite WFC0 in CNTS_CUR. clarify. }
+                subst cnt. assert (b1 = cnt_cur_b).
+                { setoid_rewrite WFC5 in FIND_CNT_CUR. clarify. }
+                subst b1. assert (b0 = cur).
+                { rewrite FIND_CUR_C in H. clarify. }
+                subst b0. assert (f0 = f).
+                { rewrite FINDF_C_CUR in H0. clarify. }
+                subst f0. erewrite Mem.load_store_same. 2: eapply CNT_CUR_STORE.
+                ss. rewrite map_length. rewrite get_id_tr_app. ss.
+                rewrite Pos.eqb_refl. rewrite app_length. ss.
+                do 2 f_equal. apply nat64_int64_add_one.
+                admit. (*ez*)
+              * ss. erewrite Mem.load_store_other. 2: eapply CNT_CUR_STORE.
+                2:{ left. ii. clarify. apply Genv.find_invert_symbol in FIND_CNT_CUR, WFC5.
+                    rewrite FIND_CNT_CUR in WFC5. clarify. rename cnt into cnt_cur.
+                    specialize (CNT_INJ _ _ _ CNTS_CUR WFC0). clarify.
+                }
+                rewrite get_id_tr_app. ss. apply Pos.eqb_neq in n. rewrite n. rewrite app_nil_r. rewrite WFC7. auto.
+
+          - move IND after cst2. move FREE after cst2. move FREEENV after cst2.
+            hexploit wunchanged_on_free_list_preserves. eapply WCHG1. all: eauto. intros WCHG2.
+            hexploit wunchanged_on_exists_mem_free_list. eapply WCHG2. eapply FREE. intros (m_c_next2 & FREE2).
+            exists m_c_next2. splits; auto.
+            hexploit wunchanged_on_free_list_preserves. eapply WCHG2. all: eauto. intros WCHG3.
+            eapply wf_c_cont_wunchanged_on. eapply IND. auto.
+
+          - move WFC2 after cst2. unfold wf_c_stmt in *. i. rewrite CNTS_NEXT in H. inv H. rename cnt into cnt_next.
+            subst f_next. unfold comp_of. ss. apply match_symbs_code_bundle_trace. destruct MS0 as (MS0 & _); auto.
+
+          - move WFNB after cst2. unfold wf_c_nb in *.
+            apply SimplLocalsproof.free_list_nextblock in FREENEXT. rewrite FREENEXT.
+            eapply mem_delta_apply_wf_wunchanged_on in DELTA_C. eapply store_wunchanged_on in CNT_CUR_STORE.
+            eapply wunchanged_on_nextblock in CNT_CUR_STORE, DELTA_C.
+            clear - WFNB CNT_CUR_STORE DELTA_C.
+            do 5 (etransitivity; eauto).
+            Unshelve. all: try (exact 0%nat). all: try (exact (fun _ _ => True)).
+        }
+
+        assert (MS_NEXT: match_state ge_i ge_c (meminj_public ge_i) ttr cnts pars id_next (Some (b, m2, ik')) cst2).
+        { clear CUR_SWITCH_STAR WFC_NEXT. ss. splits; auto.
+          - unfold match_mem. splits; auto.
+            + eapply SimplLocalsproof.free_list_right_inject. eapply MEMINJ_CNT. eapply FREENEXT.
+              i. move WFC4 after cst2. apply not_global_is_not_inj_bloks in WFC4. setoid_rewrite Forall_forall in WFC4.
+              assert (b2 = b1).
+              { clear - H. unfold meminj_public in H. des_ifs. }
+              subst b2. hexploit (WFC4 b1).
+              { unfold blocks_of_env2, blocks_of_env in *. rewrite map_map.
+                eapply (in_map (fun x => fst (fst x))) in H0. ss. rewrite map_map in H0. ss.
+              }
+              intros. erewrite <- match_symbs_meminj_public in H3. rewrite H in H3. clarify.
+              destruct MS0 as (MS & _). apply MS.
+            + move MS1 after cst2. destruct MS1 as (MM1 & MM2 & MM3).
+              move DELTA after cst2. eapply meminj_not_alloc_delta. eapply MM3. eapply DELTA.
+          - unfold match_cur_fun. splits; auto. eauto.
+          - destruct MS1 as (MM1 & MM2 & MM3). eapply mem_inject_incr_match_cnts_rev; eauto.
+        }
+        exists cst2. split.
+        2:{ left. exists id_next. split. apply WFC_NEXT. eexists. eapply MS_NEXT. }
+
+        unfold wf_c_stmt in WFC2. specialize (WFC2 _ CNTS_CUR). subst stmt.
+        eapply star_trans. eapply code_bundle_trace_spec. 2: ss.
+        unfold switch_bundle_events at 1. rewrite CUR_TR at 1. rewrite map_app. simpl.
+        rewrite ! (match_symbs_code_bundle_return ge_i ge_c) in CUR_SWITCH_STAR. rewrite ! (match_symbs_code_bundle_events ge_i ge_c) in CUR_SWITCH_STAR.
+        eapply star_trans. eapply CUR_SWITCH_STAR. 2: ss. 2,3: destruct MS0 as (MS & _); auto.
+        clear BOUND2 CUR_SWITCH_STAR.
+        unfold code_bundle_return. eapply star_trans. eapply code_mem_delta_correct. auto.
+        { erewrite <- match_symbs_mem_delta_apply_wf. eapply DELTA_C. destruct MS0 as (MSYMB & _). auto. }
+        2: ss.
+        unfold unbundle. simpl. rename b into next.
+
+        assert (CP_NEXT: (Genv.find_comp ge_c (Vptr next Ptrofs.zero)) = (comp_of fi_next)).
+        { unfold Genv.find_comp. apply Genv.find_funct_ptr_iff in FINDF_C. setoid_rewrite FINDF_C. subst f_next. ss. }
+        assert (EVRETV: eventval_to_val ge_c evretv = vretv).
+        { destruct MS0 as (MSENV & MGENV). inv TR.
+          eapply eventval_match_eventval_to_val. eapply match_symbs_eventval_match; eauto.
+        }
+
+        econs 2.
+        { inv TR. eapply match_senv_eventval_match in H0. 2: destruct MS0 as (MS0 & _); apply MS0.
+          eapply step_return_1.
+          - eapply eventval_to_expr_val_eval. auto. eapply H0.
+          - ss. assert (fd_cur = AST.Internal f_i_cur).
+            { rewrite FINDFD in FINDF_I_CUR; clarify. }
+            subst fd_cur. eapply sem_cast_proj_rettype. ss. eapply H0.
+          - eapply FREENEXT.
+        }
+        ss. econs 2.
+        { assert (CPEQ1: comp_of f_next = (Genv.find_comp ge_i (Vptr next Ptrofs.zero))).
+          { subst f_next. unfold comp_of, gen_function. ss. unfold Genv.find_comp. setoid_rewrite INTERNAL. ss. }
+          assert (CPEQ2: (comp_of (gen_function ge_i cnt_cur params_cur (get_id_tr ttr id_cur) f_i_cur)) = (Genv.find_comp ge_i (Vptr cur Ptrofs.zero))).
+          { unfold comp_of, gen_function. ss. unfold Genv.find_comp. setoid_rewrite FINDF_I_CUR. ss. }
+          eapply step_returnstate.
+          - move NPTR after EVRETV. i. rewrite EVRETV. apply NPTR. rr. rewrite CPEQ1 in H. setoid_rewrite CPEQ2 in H. apply H.
+          - move TR after EVRETV. instantiate (1:=tr). inv TR. setoid_rewrite CPEQ2. rewrite CPEQ1. econs; auto.
+            assert (fd_cur = AST.Internal f_i_cur).
+            { rewrite FINDFD in FINDF_I_CUR; clarify. }
+            subst fd_cur. ss. erewrite proj_rettype_to_type_rettype_of_type_eq. 2: eapply H0.
+            eapply match_senv_eventval_match. 2: eapply H0. destruct MS0 as (MS0 & _). auto.
+        }
+        ss. econs 2.
+        { eapply step_skip_or_continue_loop1. auto. }
+        econs 2.
+        { eapply step_skip_loop2. }
+        { subst cst2. unfold code_bundle_trace. unfold Swhile. destruct MS0 as (MS0 & _).
+          erewrite (match_symbs_switch_bundle_events _ _ MS0).
+          setoid_rewrite <- CP_NEXT. unfold Genv.find_comp. setoid_rewrite FUN.
+          replace (comp_of (Internal f_next)) with (comp_of f_next). econs 1. ss.
+        }
+        all: traceEq. traceEq.
+
+
+
+
+
+
+          TODO
+
+
+
+        assert (DELTA_C: exists m_c', (mem_delta_apply_wf ge_i (comp_of f) d (Some m_cu) = Some m_c') /\
+                                   (Mem.inject (meminj_public ge_i) m2 m_c')).
+        { move MS1 after CUR_SWITCH_STAR. destruct MS1 as (MINJ & INJINCR & NALLOC).
+          move DELTA after NALLOC. move ECCASES after DELTA. desH ECCASES; cycle 1.
+          { subst d. unfold mem_delta_apply_wf in *. ss. inv DELTA.
+
+            TODO
+
+
+          move PUB after NALLOC.
+          hexploit mem_delta_apply_establish_inject_preprocess2.
+          apply MINJ. eapply CNT_CUR_STORE.
+          { instantiate (1:=ge_i). erewrite match_symbs_meminj_public. 2: destruct MS0 as (MS & _); apply MS.
+            ii. unfold meminj_public in H. des_ifs. apply Senv.find_invert_symbol in FIND_CNT_CUR.
+            rewrite FIND_CNT_CUR in Heq. clarify.
+          }
+          apply INJINCR. apply NALLOC. apply DELTA. apply PUB.
+          intros (m_c' & DELTA' & INJ'). exists m_c'. splits; auto.
+          rewrite CP_CUR. auto.
+        }
+        des. rename DELTA_C0 into MEMINJ_CNT.
+
+        assert (WCHG1: wunchanged_on (fun b _ => Mem.valid_block m_c b) m_c m_c').
+        { eapply wunchanged_on_trans. eapply store_wunchanged_on. eapply CNT_CUR_STORE.
+          eapply wunchanged_on_implies. eapply mem_delta_apply_wf_wunchanged_on. eapply DELTA_C. ss.
+        }
+        assert (FREENEXT: exists m_c_next, Mem.free_list m_c' (blocks_of_env ge_c e) (comp_of f) = Some m_c_next).
+        { eapply wunchanged_on_exists_mem_free_list. eapply WCHG1. eapply FREEENV. }
+        des.
+
+        set (State f_next (fn_body f_next) ck_next e_next le_next m_c_next) as cst2.
+
+        assert (WFC_NEXT: wf_c_state ge_c (pretr ++ [(id_cur, Bundle_return tr evretv d)]) ttr cnts id_next cst2).
+        { clear CUR_SWITCH_STAR. ss. splits; auto.
+          - unfold wf_counters. split. auto.
+            move WFC0 after cst2.
+            ii. specialize (WFC0 _ _ _ H H0). des. exists cnt. splits; auto.
+            unfold wf_counter in WFC1. des. unfold wf_counter. splits; auto.
+            exists b1. splits; auto.
+            + eapply mem_valid_access_wunchanged_on. eapply WFC6.
+              eapply wunchanged_on_trans; cycle 1. eapply mem_free_list_wunchanged_on_2. eapply FREENEXT.
+              eapply wunchanged_on_trans; cycle 1. eapply mem_delta_apply_wf_wunchanged_on. eapply DELTA_C.
+              eapply store_wunchanged_on. eapply CNT_CUR_STORE. ss. i.
+              move MS5 after H0. destruct MS5 as (MP0 & MP1 & MP). specialize (MP _ _ WFC5). move WFC4 after MP.
+              eapply not_global_blks_global_not_in; eauto.
+            + move WFNB after CP_CUR. move WFC4 after WFNB.
+              eapply Mem.load_unchanged_on. eapply mem_free_list_unchanged_on. eapply FREENEXT.
+              { ss. i. eapply not_global_blks_global_not_in; eauto. }
+              erewrite mem_delta_apply_wf_mem_load; cycle 1.
+              { erewrite match_symbs_mem_delta_apply_wf in DELTA_C. apply DELTA_C. destruct MS0 as (MS & _). eauto. }
+              { eapply Genv.find_invert_symbol. apply WFC5. }
+              { auto. }
+              destruct (Pos.eq_dec id id_cur).
+              * subst id. assert (cnt_cur = cnt).
+                { rewrite WFC0 in CNTS_CUR. clarify. }
+                subst cnt. assert (b1 = cnt_cur_b).
+                { setoid_rewrite WFC5 in FIND_CNT_CUR. clarify. }
+                subst b1. assert (b0 = cur).
+                { rewrite FIND_CUR_C in H. clarify. }
+                subst b0. assert (f0 = f).
+                { rewrite FINDF_C_CUR in H0. clarify. }
+                subst f0. erewrite Mem.load_store_same. 2: eapply CNT_CUR_STORE.
+                ss. rewrite map_length. rewrite get_id_tr_app. ss.
+                rewrite Pos.eqb_refl. rewrite app_length. ss.
+                do 2 f_equal. apply nat64_int64_add_one.
+                admit. (*ez*)
+              * ss. erewrite Mem.load_store_other. 2: eapply CNT_CUR_STORE.
+                2:{ left. ii. clarify. apply Genv.find_invert_symbol in FIND_CNT_CUR, WFC5.
+                    rewrite FIND_CNT_CUR in WFC5. clarify. rename cnt into cnt_cur.
+                    specialize (CNT_INJ _ _ _ CNTS_CUR WFC0). clarify.
+                }
+                rewrite get_id_tr_app. ss. apply Pos.eqb_neq in n. rewrite n. rewrite app_nil_r. rewrite WFC7. auto.
+
+          - move IND after cst2. move FREE after cst2. move FREEENV after cst2.
+            hexploit wunchanged_on_free_list_preserves. eapply WCHG1. all: eauto. intros WCHG2.
+            hexploit wunchanged_on_exists_mem_free_list. eapply WCHG2. eapply FREE. intros (m_c_next2 & FREE2).
+            exists m_c_next2. splits; auto.
+            hexploit wunchanged_on_free_list_preserves. eapply WCHG2. all: eauto. intros WCHG3.
+            eapply wf_c_cont_wunchanged_on. eapply IND. auto.
+
+          - move WFC2 after cst2. unfold wf_c_stmt in *. i. rewrite CNTS_NEXT in H. inv H. rename cnt into cnt_next.
+            subst f_next. unfold comp_of. ss. apply match_symbs_code_bundle_trace. destruct MS0 as (MS0 & _); auto.
+
+          - move WFNB after cst2. unfold wf_c_nb in *.
+            apply SimplLocalsproof.free_list_nextblock in FREENEXT. rewrite FREENEXT.
+            eapply mem_delta_apply_wf_wunchanged_on in DELTA_C. eapply store_wunchanged_on in CNT_CUR_STORE.
+            eapply wunchanged_on_nextblock in CNT_CUR_STORE, DELTA_C.
+            clear - WFNB CNT_CUR_STORE DELTA_C.
+            do 5 (etransitivity; eauto).
+            Unshelve. all: try (exact 0%nat). all: try (exact (fun _ _ => True)).
+        }
+
+        assert (MS_NEXT: match_state ge_i ge_c (meminj_public ge_i) ttr cnts pars id_next (Some (b, m2, ik')) cst2).
+        { clear CUR_SWITCH_STAR WFC_NEXT. ss. splits; auto.
+          - unfold match_mem. splits; auto.
+            + eapply SimplLocalsproof.free_list_right_inject. eapply MEMINJ_CNT. eapply FREENEXT.
+              i. move WFC4 after cst2. apply not_global_is_not_inj_bloks in WFC4. setoid_rewrite Forall_forall in WFC4.
+              assert (b2 = b1).
+              { clear - H. unfold meminj_public in H. des_ifs. }
+              subst b2. hexploit (WFC4 b1).
+              { unfold blocks_of_env2, blocks_of_env in *. rewrite map_map.
+                eapply (in_map (fun x => fst (fst x))) in H0. ss. rewrite map_map in H0. ss.
+              }
+              intros. erewrite <- match_symbs_meminj_public in H3. rewrite H in H3. clarify.
+              destruct MS0 as (MS & _). apply MS.
+            + move MS1 after cst2. destruct MS1 as (MM1 & MM2 & MM3).
+              move DELTA after cst2. eapply meminj_not_alloc_delta. eapply MM3. eapply DELTA.
+          - unfold match_cur_fun. splits; auto. eauto.
+        }
+        exists cst2. split.
+        2:{ left. exists id_next. split. apply WFC_NEXT. eexists. eapply MS_NEXT. }
+
+        unfold wf_c_stmt in WFC2. specialize (WFC2 _ CNTS_CUR). subst stmt.
+        eapply star_trans. eapply code_bundle_trace_spec. 2: ss.
+        unfold switch_bundle_events at 1. rewrite CUR_TR at 1. rewrite map_app. simpl.
+        rewrite ! (match_symbs_code_bundle_return ge_i ge_c) in CUR_SWITCH_STAR. rewrite ! (match_symbs_code_bundle_events ge_i ge_c) in CUR_SWITCH_STAR.
+        eapply star_trans. eapply CUR_SWITCH_STAR. 2: ss. 2,3: destruct MS0 as (MS & _); auto.
+        clear BOUND2 CUR_SWITCH_STAR.
+        unfold code_bundle_return. eapply star_trans. eapply code_mem_delta_correct. auto.
+        { erewrite <- match_symbs_mem_delta_apply_wf. eapply DELTA_C. destruct MS0 as (MSYMB & _). auto. }
+        2: ss.
+        unfold unbundle. simpl. rename b into next.
+
+        assert (CP_NEXT: (Genv.find_comp ge_c (Vptr next Ptrofs.zero)) = (comp_of fi_next)).
+        { unfold Genv.find_comp. apply Genv.find_funct_ptr_iff in FINDF_C. setoid_rewrite FINDF_C. subst f_next. ss. }
+        assert (EVRETV: eventval_to_val ge_c evretv = vretv).
+        { destruct MS0 as (MSENV & MGENV). inv TR.
+          eapply eventval_match_eventval_to_val. eapply match_symbs_eventval_match; eauto.
+        }
+
+        econs 2.
+        { inv TR. eapply match_senv_eventval_match in H0. 2: destruct MS0 as (MS0 & _); apply MS0.
+          eapply step_return_1.
+          - eapply eventval_to_expr_val_eval. auto. eapply H0.
+          - ss. assert (fd_cur = AST.Internal f_i_cur).
+            { rewrite FINDFD in FINDF_I_CUR; clarify. }
+            subst fd_cur. eapply sem_cast_proj_rettype. ss. eapply H0.
+          - eapply FREENEXT.
+        }
+        ss. econs 2.
+        { assert (CPEQ1: comp_of f_next = (Genv.find_comp ge_i (Vptr next Ptrofs.zero))).
+          { subst f_next. unfold comp_of, gen_function. ss. unfold Genv.find_comp. setoid_rewrite INTERNAL. ss. }
+          assert (CPEQ2: (comp_of (gen_function ge_i cnt_cur params_cur (get_id_tr ttr id_cur) f_i_cur)) = (Genv.find_comp ge_i (Vptr cur Ptrofs.zero))).
+          { unfold comp_of, gen_function. ss. unfold Genv.find_comp. setoid_rewrite FINDF_I_CUR. ss. }
+          eapply step_returnstate.
+          - move NPTR after EVRETV. i. rewrite EVRETV. apply NPTR. rr. rewrite CPEQ1 in H. setoid_rewrite CPEQ2 in H. apply H.
+          - move TR after EVRETV. instantiate (1:=tr). inv TR. setoid_rewrite CPEQ2. rewrite CPEQ1. econs; auto.
+            assert (fd_cur = AST.Internal f_i_cur).
+            { rewrite FINDFD in FINDF_I_CUR; clarify. }
+            subst fd_cur. ss. erewrite proj_rettype_to_type_rettype_of_type_eq. 2: eapply H0.
+            eapply match_senv_eventval_match. 2: eapply H0. destruct MS0 as (MS0 & _). auto.
+        }
+        ss. econs 2.
+        { eapply step_skip_or_continue_loop1. auto. }
+        econs 2.
+        { eapply step_skip_loop2. }
+        { subst cst2. unfold code_bundle_trace. unfold Swhile. destruct MS0 as (MS0 & _).
+          erewrite (match_symbs_switch_bundle_events _ _ MS0).
+          setoid_rewrite <- CP_NEXT. unfold Genv.find_comp. setoid_rewrite FUN.
+          replace (comp_of (Internal f_next)) with (comp_of f_next). econs 1. ss.
+        }
+        all: traceEq. traceEq.
+
+
+        TODO
         
 
 
